[Micheline] Micheline parser

src/michocoq/micheline_parser.vy
@@ -1,0 +1,51 @@
+%{Require Import String ZArith.
+Require Import micheline_syntax.
+%}
+
+%token LBRACE RBRACE SEMICOLON LPAREN RPAREN
+%token <string> PRIM STR BYTES
+%token <Z> NUMBER
+%token EOF
+
+%start <micheline> file
+
+%type <list micheline> seq args
+%type <micheline> arg atom app micheline
+
+%%
+
+atom:
+    STR { STR $1 }
+  | BYTES { BYTES $1 }
+  | NUMBER { NUMBER $1 }
+  | LBRACE seq RBRACE { SEQ $2 }
+;
+
+arg:
+    atom { $1 }
+  | LPAREN app RPAREN { $2 }
+  | PRIM { PRIM $1 nil }
+;
+
+args:
+    arg { cons $1 nil }
+  | arg args { cons $1 $2 }
+;
+
+micheline:
+    atom { $1 }
+  | PRIM { PRIM $1 nil }
+  | app { $1 }
+;
+
+seq:
+    { nil }
+  | micheline SEMICOLON seq { cons $1 $3 }
+;
+
+app:
+    PRIM args { PRIM $1 $2 }
+;
+
+file: micheline EOF { $1 }
+%%
