src/michocoq/main.v
@@ -1,0 +1,16 @@
+Require Import String ZArith.
+Require micheline_lexer micheline_parser.
+
+Definition lex_and_parse_micheline (fuel : nat) (input : string)
+  : error.M micheline_syntax.micheline :=
+  error.bind
+    (fun s =>
+       match micheline_parser.file fuel s with
+       | micheline_parser.Parser.Inter.Fail_pr =>
+         error.Failed _ error.Parsing
+       | micheline_parser.Parser.Inter.Timeout_pr =>
+         error.Failed _ error.Parsing_Out_of_Fuel
+       | micheline_parser.Parser.Inter.Parsed_pr m _ =>
+         error.Return _ m
+       end)
+    (micheline_lexer.lex_micheline_to_parser input).
