src/michocoq/micheline_syntax.v
@@ -1,0 +1,8 @@
+Require Import String ZArith.
+
+Inductive micheline :=
+| SEQ (_ : list micheline)
+| PRIM (_ : string) (_ : list micheline)
+| STR (_ : string)
+| BYTES (_ : string)
+| NUMBER (_ : Z).
