src/michocoq/micheline_tokens.v
@@ -1,0 +1,57 @@
+Require Import String ZArith.
+Require micheline_parser.
+Import micheline_parser.Aut.GramDefs.
+
+(** Tokens *)
+Inductive token :=
+| LBRACE
+| RBRACE
+| SEMICOLON
+| LPAREN
+| RPAREN
+| PRIM : string -> token
+| STR : string -> token
+| NUMBER : Z -> token
+| BYTES : string -> token
+| EOF.
+
+Definition parser_token := micheline_parser.Aut.GramDefs.token.
+
+Definition token_from_parser (t : parser_token) : token :=
+  match t with
+  | existT _ LBRACE't tt => LBRACE
+  | existT _ RBRACE't tt => RBRACE
+  | existT _ SEMICOLON't tt => SEMICOLON
+  | existT _ LPAREN't tt => LPAREN
+  | existT _ RPAREN't tt => RPAREN
+  | existT _ PRIM't s => PRIM s
+  | existT _ STR't s => STR s
+  | existT _ NUMBER't n => NUMBER n
+  | existT _ BYTES't s => BYTES s
+  | existT _ EOF't tt => EOF
+  end.
+
+Definition token_to_parser (t : token) : parser_token :=
+  match t with
+  | LBRACE => existT _ LBRACE't tt
+  | RBRACE => existT _ RBRACE't tt
+  | SEMICOLON => existT _ SEMICOLON't tt
+  | LPAREN => existT _ LPAREN't tt
+  | RPAREN => existT _ RPAREN't tt
+  | PRIM s => existT _ PRIM't s
+  | STR s => existT _ STR't s
+  | NUMBER n => existT _ NUMBER't n
+  | BYTES s => existT _ BYTES't s
+  | EOF => existT _ EOF't tt
+  end.
+
+Lemma token_to_parser_from_parser t : token_to_parser (token_from_parser t) = t.
+Proof.
+  destruct t as (terminal, semantic).
+  destruct terminal; try reflexivity; destruct semantic; reflexivity.
+Qed.
+
+Lemma token_from_parser_to_parser t : token_from_parser (token_to_parser t) = t.
+Proof.
+  destruct t; reflexivity.
+Qed.
